simpifying LR for closed types only + closed type dervtns + other..

theories/backtranslation/cast_help/between.v
@@ -1,5 +1,6 @@
 From fae_gtlc_mu.stlc_mu Require Export typing lang lib.fix.
 From fae_gtlc_mu Require Export prelude.
+From Coq Require Export List.
 
 (** Between sums, products, recursive types, arrow types *)
 
@@ -14,7 +15,7 @@ Proof.
 Qed.
 
 Definition between_TSum (c1 c2 : expr) : val :=
-  LamV (Case (Var 0) (InjL ((rename (+2) c1) (Var 0))) (InjR ((rename (+2) c2) (Var 0)))).
+  LamV (Case (Var 0) (InjL ((c1.[ren (+2)]) (Var 0))) (InjR ((c2.[ren (+2)]) (Var 0)))).
 
 Lemma between_TSum_subst_rewrite σ f1 f2 :
   (# (between_TSum f1 f2)).[σ] =
@@ -24,21 +25,24 @@ Proof.
   by asimpl.
 Qed.
 
-Lemma between_TSum_typed Γ (τ1 τ2 τ1' τ2' : type) (f1 f2 : expr) (d1 : Γ ⊢ₛ f1 : (TArrow τ1 τ1')) (d2 : Γ ⊢ₛ f2 : (TArrow τ2 τ2')) :
-  Γ ⊢ₛ between_TSum f1 f2 : (TArrow (τ1 + τ2) (τ1' + τ2'))%type.
+Lemma between_TSum_typed Γ pΓ τ1 pτ1 τ2 pτ2 τ1' pτ1' τ2' pτ2' (f1 f2 : expr)
+      (d1 : Γ & pΓ ⊢ₛ f1 : (TArrow τ1 τ1') & (TArrow_closed pτ1 pτ1'))
+      (d2 : Γ & pΓ ⊢ₛ f2 : (TArrow τ2 τ2') & (TArrow_closed pτ2 pτ2')) :
+  Γ & pΓ ⊢ₛ between_TSum f1 f2 : (TArrow (τ1 + τ2) (τ1' + τ2'))%type & (TArrow_closed (TSum_closed pτ1 pτ2) (TSum_closed pτ1' pτ2')).
 Proof.
-  apply Lam_typed.
+  eapply Lam_typed.
   eapply Case_typed.
   by apply Var_typed.
-  constructor. eapply App_typed.
-  apply up_type_two. apply d1.
+  eapply InjL_typed. eapply App_typed.
+  eapply up_type_two. apply d1.
   by apply Var_typed.
-  constructor. eapply App_typed.
-  apply up_type_two. apply d2. by apply Var_typed.
+  eapply InjR_typed. eapply App_typed.
+  eapply up_type_two. apply d2. by apply Var_typed.
+  Unshelve. all:intro σ; asimpl; repeat rewrite pτ1; repeat rewrite pτ1'; repeat rewrite pτ2; repeat rewrite pτ2'; done.
 Qed.
 
 Definition between_TProd (f1 f2 : expr) : val :=
-  LamV (Pair (rename (+1) f1 (Fst (Var 0))) (rename (+1) f2 (Snd (Var 0)))).
+  LamV (Pair (f1.[ren (+1)] (Fst (Var 0))) (f2.[ren (+1)] (Snd (Var 0)))).
 
 Lemma between_TProd_subst_rewrite σ f1 f2 :
   (# (between_TProd f1 f2)).[σ] =
@@ -48,21 +52,24 @@ Proof.
   by asimpl.
 Qed.
 
-Lemma between_TProd_typed Γ (τ1 τ2 τ1' τ2' : type) (f1 f2 : expr) (d1 : Γ ⊢ₛ f1 : (TArrow τ1 τ1')) (d2 : Γ ⊢ₛ f2 : (TArrow τ2 τ2')) :
-  Γ ⊢ₛ between_TProd f1 f2 : (TArrow (τ1 × τ2) (τ1' × τ2'))%type.
+Lemma between_TProd_typed Γ pΓ τ1 pτ1 τ2 pτ2 τ1' pτ1' τ2' pτ2' (f1 f2 : expr)
+      (d1 : Γ & pΓ ⊢ₛ f1 : (TArrow τ1 τ1') & (TArrow_closed pτ1 pτ1'))
+      (d2 : Γ & pΓ ⊢ₛ f2 : (TArrow τ2 τ2') & (TArrow_closed pτ2 pτ2')) :
+  Γ & pΓ ⊢ₛ between_TProd f1 f2 : (TArrow (τ1 × τ2) (τ1' × τ2'))%type & (TArrow_closed (TProd_closed pτ1 pτ2) (TProd_closed pτ1' pτ2')).
 Proof.
-  apply Lam_typed.
-  apply Pair_typed.
+  eapply Lam_typed.
+  eapply Pair_typed.
   eapply App_typed.
-  apply up_type_one. apply d1. econstructor. by apply Var_typed.
+  eapply up_type_one. apply d1. econstructor. by apply Var_typed.
   eapply App_typed.
   apply up_type_one. apply d2. econstructor. by apply Var_typed.
+  Unshelve. all:intro σ; asimpl; repeat rewrite pτ1; repeat rewrite pτ1'; repeat rewrite pτ2; repeat rewrite pτ2'; done.
 Qed.
 
 Definition between_TArrow (ca cr : expr) : val :=
   LamV (*f*)
     (Lam (*a*) (
-         rename (+2) cr (((Var 1)(*f*)) (rename (+2) ca (Var 0(*a*))))
+         cr.[ren (+2)] (((Var 1)(*f*)) (ca.[ren (+2)] (Var 0(*a*))))
        )
     ).
 
@@ -74,23 +81,27 @@ Proof.
   by asimpl.
 Qed.
 
-Lemma between_TArrow_typed Γ (τ1 τ2 τ3 τ4 : type) (ca cr : expr) (da : Γ ⊢ₛ ca : (TArrow τ3 τ1)) (dr : Γ ⊢ₛ cr : (TArrow τ2 τ4)) :
-  Γ ⊢ₛ between_TArrow ca cr : (TArrow (TArrow τ1 τ2) (TArrow τ3 τ4))%type.
+Lemma between_TArrow_typed Γ pΓ τ1 pτ1 τ2 pτ2 τ3 pτ3 τ4 pτ4 (ca cr : expr)
+      (da : Γ & pΓ ⊢ₛ ca : (TArrow τ3 τ1) & (TArrow_closed pτ3 pτ1))
+      (dr : Γ & pΓ ⊢ₛ cr : (TArrow τ2 τ4) & (TArrow_closed pτ2 pτ4)) :
+  Γ & pΓ ⊢ₛ between_TArrow ca cr : (TArrow (TArrow τ1 τ2) (TArrow τ3 τ4))%type &
+                                   (TArrow_closed (TArrow_closed pτ1 pτ2) (TArrow_closed pτ3 pτ4)).
 Proof.
-  repeat apply Lam_typed.
-  apply App_typed with (τ1 := τ2).
-  auto. apply up_type_two. apply dr. apply App_typed with (τ1 := τ1).
+  repeat eapply Lam_typed.
+  eapply App_typed with (τ1 := τ2).
+  eapply up_type_two. apply dr. eapply App_typed with (τ1 := τ1).
     by auto; apply Var_typed.
-    eapply App_typed. by apply up_type_two.
+    eapply App_typed. by eapply up_type_two.
     by apply Var_typed.
+  Unshelve. all:intro σ; asimpl; repeat rewrite pτ1; repeat rewrite pτ2; repeat rewrite pτ3; repeat rewrite pτ4; done.
 Qed.
 
 Definition between_TRec (f : expr) : val :=
   LamV (* x : μ. τi *) (
-      Fix'' (
+      Fix (
           Lam (* g : μ.τi → μ.τf *) (
               Lam (* r : μ.τi *) (
-                  Fold (rename (+1) (f.[upn 1 (ren (+ 1))])(* : τi.[μ.τi/] → τf.[μ.τf]*) (Unfold (Var 0)))
+                  Fold (f.[upn 1 (ren (+ 1))].[ren (+1)](* : τi.[μ.τi/] → τf.[μ.τf]*) (Unfold (Var 0)))
                 )
             )
         ) (Var 0)
@@ -103,7 +114,7 @@ Proof.
   rewrite /between_TRec.
   rewrite subst_lam.
   rewrite subst_app.
-  rewrite Fix''_subs_rewrite.
+  rewrite Fix_subs_rewrite.
   by asimpl.
 Qed.
 
@@ -114,25 +125,33 @@ Proof.
   by simpl.
 Qed.
 
-Lemma between_TRec_typed Γ (τi τf : type) (Pi : Is_Closed (TRec τi)) (Pf : Is_Closed (TRec τf)) (f : expr)
-      (d : ((TArrow (TRec τi) (TRec τf)):: Γ) ⊢ₛ f : (TArrow (τi.[TRec τi/]) τf.[TRec τf/])) :
-  Γ ⊢ₛ between_TRec f : (TArrow (stlc_mu.typing.TRec τi) (stlc_mu.typing.TRec τf))%type.
+Lemma between_TRec_typed Γ pΓ τi pμτi τf pμτf (f : expr)
+      (d : ((TArrow (TRec τi) (TRec τf)):: Γ) & (Forall_cons _ _ _ (TArrow_closed pμτi pμτf) pΓ) ⊢ₛ f : (TArrow (τi.[TRec τi/]) τf.[TRec τf/]) &
+      TArrow_closed (TRec_closed_unfold pμτi) (TRec_closed_unfold pμτf)) :
+  Γ & pΓ ⊢ₛ between_TRec f : (TArrow (TRec τi) (TRec τf))%type &
+      TArrow_closed pμτi pμτf.
 Proof.
-  apply Lam_typed.
-  apply App_typed with (τ1 := TRec τi).
-  apply Fix''_typed; auto.
-    (* by intro τ; simpl; rewrite -(Pi τ); rewrite -(Pf τ); by simpl. *)
-  apply Lam_typed.
-  apply Lam_typed.
-  apply Fold_typed.
-  apply App_typed with (τ1 := τi.[(TRec τi)/]).
-  apply up_type_one.
-  rewrite rewrite_for_context_weakening in d.
+  eapply Lam_typed.
+  eapply App_typed with (τ1 := TRec τi).
+  apply Fix_typed; auto.
+  eapply Lam_typed.
+  eapply Lam_typed.
+  eapply Fold_typed.
+  eapply App_typed with (τ1 := τi.[(TRec τi)/]).
+  eapply up_type_one.
+  revert d.
+  generalize (Forall_cons TClosed (TArrow (TRec τi) (TRec τf)) Γ (TArrow_closed pμτi pμτf) pΓ).
+  rewrite rewrite_for_context_weakening. intros pp d.
+  Unshelve. 4-15: auto. 4-5: by apply TArrow_closed.
+  generalize (Forall_cons TClosed (TArrow (TRec τi) (TRec τf)) (TRec τi :: Γ) (TArrow_closed pμτi pμτf)
+    (Forall_cons TClosed (TRec τi) Γ pμτi pΓ)).
   rewrite (rewrite_for_context_weakening Γ).
   rewrite rewrite_for_context_weakening.
-  apply context_gen_weakening.
+  intro ppp.
+  eapply context_gen_weakening.
   apply d.
-  apply Unfold_typed.
+  eapply Unfold_typed.
   by apply Var_typed.
   by apply Var_typed.
+  Unshelve. all: try done; by apply TRec_closed_unfold.
 Qed.
