theories/backtranslation/cast_help/general.v
@@ -1,19 +1,19 @@
 From fae_gtlc_mu.stlc_mu Require Export typing lang lib.fix.
-From fae_gtlc_mu.cast_calculus Require Export types consistency.structural.definition.
+From fae_gtlc_mu.cast_calculus Require Export types consistency.structural.
 From fae_gtlc_mu.backtranslation.cast_help Require Export universe embed extract between factorize.
-(* From fae_gtlc_mu.backtranslation Require Export types de_bruijn_hell. *)
+From Coq Require Export List.
 
 (** emulation of a cast between an arbitrary pair of consistent types *)
 (* recursively defined on the alternative consistency relation *)
 
-Fixpoint 𝓕 {A : list (types.type * types.type)} {τi τf : cast_calculus.types.type} (P : A ⊢ τi ~ τf) : expr :=
+Fixpoint 𝓕 {A : list (types.type * types.type)} {τi τf : cast_calculus.types.type} (P : cons_struct A τi τf) : expr :=
   match P with
   | consStarTGround _ τG G => extract τG G
   | consTGroundStar _ τG G => embed τG G
-  | consTauStar _ τ τG pτnG pτnStar pτSτG pτConsτG =>
+  | consTauStar _ τ τG pτnG pτnStar pτSτG pτConsτG pτGConsStar =>
     factorization_up
       (𝓕 pτConsτG) τG (get_shape_is_ground pτSτG)
-  | consStarTau _ τ τG pτnG pτnStar pτSτG pτGConsτ =>
+  | consStarTau _ τ τG pτnG pτnStar pτSτG pStarConsτG pτGConsτ =>
     factorization_down
       (𝓕 pτGConsτ) τG (get_shape_is_ground pτSτG)
   | consBaseBase _ => identity
@@ -37,51 +37,77 @@ Fixpoint 𝓕 {A : list (types.type * types.type)} {τi τf : cast_calculus.type
   | consTRecTRecUseCall _ τl τr i pμτlμtrinA => Var i
   end.
 
-From fae_gtlc_mu.stlc_mu Require Export typing lang lib.fix.
+(* From fae_gtlc_mu.stlc_mu Require Export typing lang lib.fix. *)
 
-Definition pair_to_static_function (p : cast_calculus.types.type * cast_calculus.types.type) : stlc_mu.typing.type :=
+Definition back_pair (p : cast_calculus.types.type * cast_calculus.types.type) : stlc_mu.types.type :=
   TArrow <<p.1>> <<p.2>>.
 
-Lemma 𝓕_typed (A : list (cast_calculus.types.type * cast_calculus.types.type)) (τi τf : cast_calculus.types.type) (pτi : TClosed τi) (pτf : TClosed τf) (pτiConsτf : A ⊢ τi ~ τf) :
-  (map pair_to_static_function A) ⊢ₛ (𝓕 pτiConsτf) : (TArrow <<τi>> <<τf>>).
+Definition PTClosed (p : cast_calculus.types.type * cast_calculus.types.type) : Prop :=
+  cast_calculus.types.TClosed p.1 ∧ cast_calculus.types.TClosed p.2.
+
+Lemma back_pair_closed p : PTClosed p → TClosed (back_pair p).
 Proof.
-  induction pτiConsτf; simpl.
+  destruct p as [τ1 τ2]. intro H. destruct H as [a b].
+  apply TArrow_closed; by apply back_closed.
+Qed.
+
+Lemma Forall_fmap_impl {A B : Type} (f : A → B) (X : list A) (P : A → Prop) (Q : B → Prop)
+      (Himpl : forall a : A, P a → Q (f a)) (HP : Forall P X) : Forall Q (f <$> X).
+Proof. induction X. apply Forall_nil. inversion HP. apply Forall_cons. auto. by apply IHX. Qed.
+
+Lemma 𝓕_typed (A : list (cast_calculus.types.type * cast_calculus.types.type)) (pA : Forall (fun p => cast_calculus.types.TClosed p.1 ∧ cast_calculus.types.TClosed p.2) A)
+      (τi τf : cast_calculus.types.type) (pτi : cast_calculus.types.TClosed τi) (pτf : cast_calculus.types.TClosed τf) (pτiConsτf : cons_struct A τi τf) :
+  (map back_pair A) & Forall_fmap_impl _ _ _ _ back_pair_closed pA ⊢ₛ (𝓕 pτiConsτf) : (TArrow <<τi>> <<τf>>) &
+                                                                                       TArrow_closed (back_closed pτi) (back_closed pτf).
+Proof.
+  induction pτiConsτf; eapply PI_typed.
   - apply extract_typed.
   - apply embed_typed.
-  - apply factorization_up_typed.
-    apply IHpτiConsτf.
-    done. admit.
-  - apply factorization_down_typed.
-    apply IHpτiConsτf.
-    admit. admit.
+  - apply factorization_up_typed. eapply PI_typed.
+    apply IHpτiConsτf1.
+  - apply factorization_down_typed. eapply PI_typed.
+    apply IHpτiConsτf2.
   - apply identity_typed.
   - apply identity_typed.
   - apply between_TSum_typed.
-    apply IHpτiConsτf1.
-    admit. admit.
-    apply IHpτiConsτf2.
-    admit. admit.
+    (* fold (backtranslate_type τ1). fold (backtranslate_type τ1'). fold (𝓕 pτiConsτf1). *)
+    apply IHpτiConsτf1. apply IHpτiConsτf2.
   - apply between_TProd_typed.
     apply IHpτiConsτf1.
-    admit. admit.
     apply IHpτiConsτf2.
-    admit. admit.
   - apply between_TArrow_typed.
     apply IHpτiConsτf1.
-    admit. admit.
     apply IHpτiConsτf2.
-    admit. admit.
-  - apply between_TRec_typed.
-    admit. admit.
-    rewrite map_cons in IHpτiConsτf.
-    repeat rewrite unfolding_backtranslation_commutes in IHpτiConsτf.
+  - apply between_TRec_typed with (pμτi := back_closed pτi) (pμτf := back_closed pτf).
+    fold (backtranslate_type τl). fold (backtranslate_type τr). fold (𝓕 pτiConsτf).
+    assert (eq : TArrow (TRec << τl >>) (TRec << τr >>) :: map back_pair A = map back_pair ((types.TRec τl, types.TRec τr) :: A)). { by simpl. }
+    assert (eq' : TArrow (<< τl >>).[TRec << τl >>/] (<< τr >>).[TRec << τr >>/] = TArrow << τl.[types.TRec τl/] >> << τr.[types.TRec τr/] >>). { by repeat rewrite back_unfold_comm. }
+    cut (forall pΓ pτ, TArrow (TRec << τl >>) (TRec << τr >>) :: map back_pair A & pΓ ⊢ₛ 𝓕 pτiConsτf : TArrow (<< τl >>).[TRec << τl >>/] (<< τr >>).[TRec << τr >>/] & pτ). auto.
+    rewrite eq eq'.
+    intros.
+    eapply PI_typed. eapply PI_Γ_typed.
     apply IHpτiConsτf.
-    admit. admit.
   - apply Var_typed.
     rewrite list_lookup_fmap.
     by rewrite pμτlμtrinA.
-Admitted.
-
+    Unshelve. all:try done; try cast_calculus.types.closed_solver; try by repeat apply back_closed.
+    + apply TArrow_closed; by apply back_closed.
+    + apply Ground_closed. by eapply get_shape_is_ground.
+    + apply Ground_closed. by eapply get_shape_is_ground.
+    + by eapply cast_calculus.types.TSum_closed1.
+    + by eapply cast_calculus.types.TSum_closed1.
+    + by eapply cast_calculus.types.TSum_closed2.
+    + by eapply cast_calculus.types.TSum_closed2.
+    + by eapply cast_calculus.types.TProd_closed1.
+    + by eapply cast_calculus.types.TProd_closed1.
+    + by eapply cast_calculus.types.TProd_closed2.
+    + by eapply cast_calculus.types.TProd_closed2.
+    + by eapply cast_calculus.types.TArrow_closed2.
+    + by eapply cast_calculus.types.TArrow_closed2.
+    + constructor. simpl. split; auto. auto.
+    + by apply cast_calculus.types.TRec_closed_unfold.
+    + by apply cast_calculus.types.TRec_closed_unfold.
+Qed.
 
 Definition 𝓕c {A} {τi τf} (pC : cons_struct A τi τf) fs : stlc_mu.lang.expr :=
   (𝓕 pC).[stlc_mu.typing.env_subst fs].
@@ -100,9 +126,9 @@ Proof.
   destruct pC.
   - rewrite /𝓕c /𝓕. by rewrite extract_no_subs to_of_val.
   - rewrite /𝓕c /𝓕. by rewrite embed_no_subs to_of_val.
-  - rewrite /𝓕c /𝓕. rewrite factorization_up_subst_rewrite. fold (𝓕 pC).
+  - rewrite /𝓕c /𝓕. rewrite factorization_up_subst_rewrite. fold (𝓕 pC1).
     by rewrite to_of_val.
-  - rewrite /𝓕c /𝓕. rewrite factorization_down_subst_rewrite. fold (𝓕 pC).
+  - rewrite /𝓕c /𝓕. rewrite factorization_down_subst_rewrite. fold (𝓕 pC2).
     by rewrite to_of_val.
   - rewrite /𝓕c /𝓕. by asimpl.
   - rewrite /𝓕c /𝓕. by asimpl.
@@ -127,42 +153,65 @@ Proof.
     lia.
 Qed.
 
+
+From fae_gtlc_mu.stlc_mu Require Export lang.
+
+Lemma 𝓕c_closed_gen {A} {τi τf} (pC : cons_struct A τi τf) fs (Hfsc : Forall VClosed fs) :
+  forall n, (length A = n + length fs) → forall σ, (𝓕 pC).[upn n (env_subst fs)].[upn n σ] = (𝓕 pC).[upn n (env_subst fs)].
+Proof.
+  generalize dependent fs.
+  induction pC; intros fs Hfsc; rewrite /𝓕c /𝓕; intros n H.
+  - intro. by repeat rewrite extract_no_subs.
+  - intro. by repeat rewrite embed_no_subs.
+  - fold (𝓕 pC1). rewrite factorization_up_subst_rewrite.
+    intro. simpl. rewrite embed_no_subs.
+    assert (triv : (𝓕 pC1).[upn n (env_subst fs)].[ren (+1)].[up (upn n σ)] = (𝓕 pC1).[upn n (env_subst fs)].[(upn n σ)].[ren (+1)]). by asimpl.
+    rewrite triv. rewrite IHpC1; auto.
+  - fold (𝓕 pC2). rewrite factorization_down_subst_rewrite.
+    intro. simpl. rewrite extract_no_subs.
+    assert (triv : (𝓕 pC2).[upn n (env_subst fs)].[ren (+1)].[up (upn n σ)] = (𝓕 pC2).[upn n (env_subst fs)].[(upn n σ)].[ren (+1)]). by asimpl.
+    rewrite triv. rewrite IHpC2; auto.
+  - intro; by asimpl.
+  - intro; by asimpl.
+  - fold (𝓕 pC1). fold (𝓕 pC2). intro σ.
+    cut ((# between_TSum (𝓕 pC1) (𝓕 pC2)).[upn n (env_subst fs) >> upn n σ] = (# between_TSum (𝓕 pC1) (𝓕 pC2)).[upn n (env_subst fs)]).
+    by asimpl.
+    do 2 rewrite between_TSum_subst_rewrite.
+    rewrite -(IHpC1 _ _ _ _ σ); auto.
+    rewrite -(IHpC2 _ _ _ _ σ); auto. by asimpl.
+  - fold (𝓕 pC1). fold (𝓕 pC2). intro σ.
+    cut ((# between_TProd (𝓕 pC1) (𝓕 pC2)).[upn n (env_subst fs) >> upn n σ] = (# between_TProd (𝓕 pC1) (𝓕 pC2)).[upn n (env_subst fs)]).
+    by asimpl.
+    do 2 rewrite between_TProd_subst_rewrite.
+    rewrite -(IHpC1 _ _ _ _ σ); auto.
+    rewrite -(IHpC2 _ _ _ _ σ); auto. by asimpl.
+  - fold (𝓕 pC1). fold (𝓕 pC2). intro σ.
+    cut ((# between_TArrow (𝓕 pC1) (𝓕 pC2)).[upn n (env_subst fs) >> upn n σ] = (# between_TArrow (𝓕 pC1) (𝓕 pC2)).[upn n (env_subst fs)]).
+    by asimpl.
+    do 2 rewrite between_TArrow_subst_rewrite.
+    rewrite -(IHpC1 _ _ _ _ σ); auto.
+    rewrite -(IHpC2 _ _ _ _ σ); auto. by asimpl.
+  - fold (𝓕 pC). intro σ.
+    cut ((# between_TRec (𝓕 pC)).[upn n (env_subst fs) >> upn n σ] = (# between_TRec (𝓕 pC)).[upn n (env_subst fs)]). by asimpl.
+    do 2 rewrite between_TRec_subst_rewrite.
+    cut (# between_TRec (𝓕 pC).[upn (S n) (env_subst fs)].[upn (S n) σ] = # between_TRec (𝓕 pC).[upn (S n) (env_subst fs)]). by asimpl.
+    rewrite IHpC; auto. simpl. lia.
+  - intro σ. asimpl.
+    destruct (iter_up_cases i n (env_subst fs)) as [[-> eq] | [j [-> ->]]].
+    + asimpl. by rewrite upn_lt.
+    + assert (Hnj : n + j < length A). apply lookup_lt_is_Some. by econstructor. rewrite H in Hnj.
+      assert (Hj : j < length fs). lia.
+      destruct (fs !! j) eqn:Hf.
+      * rewrite (env_subst_lookup fs _ v).
+        assert (vc : EClosed v). apply ve_closed. eapply (Forall_lookup_1). apply Hfsc. apply Hf.
+        asimpl. by do 2 rewrite vc. auto.
+      * assert (length fs ≤ j). by apply lookup_ge_None_1. exfalso; lia.
+Qed.
+
+
 Lemma 𝓕c_closed {A} {τi τf} (pC : cons_struct A τi τf) fs (H : length A = length fs) (Hfsc : Forall VClosed fs) :
   EClosed (𝓕c pC fs).
 Proof.
-  generalize dependent fs.
-  induction pC; intros fs Hfs Hfsc; rewrite /𝓕c /𝓕.
-  - intro. by repeat rewrite extract_no_subs.
-  - intro. by repeat rewrite embed_no_subs.
-  - fold (𝓕 pC). rewrite factorization_up_subst_rewrite. fold (𝓕c pC fs).
-    intro. asimpl. rewrite embed_no_subs. by repeat rewrite IHpC.
-  - fold (𝓕 pC). rewrite factorization_down_subst_rewrite. fold (𝓕c pC fs).
-    intro. asimpl. rewrite extract_no_subs. by repeat rewrite IHpC.
-  - intro; by asimpl.
-  - intro; by asimpl.
-  - fold (𝓕 pC1). fold (𝓕 pC2).
-    rewrite between_TSum_subst_rewrite.
-    fold (𝓕c pC1 fs). fold (𝓕c pC2 fs).
-    intro; asimpl. repeat rewrite IHpC1; by repeat rewrite IHpC2.
-  - fold (𝓕 pC1). fold (𝓕 pC2).
-    rewrite between_TProd_subst_rewrite.
-    fold (𝓕c pC1 fs). fold (𝓕c pC2 fs).
-    intro; asimpl. repeat rewrite IHpC1; by repeat rewrite IHpC2.
-  - fold (𝓕 pC1). fold (𝓕 pC2).
-    rewrite between_TArrow_subst_rewrite.
-    fold (𝓕c pC1 fs). fold (𝓕c pC2 fs).
-    intro; asimpl. repeat rewrite IHpC1; by repeat rewrite IHpC2.
-  - fold (𝓕 pC).
-    rewrite between_TRec_subst_rewrite.
-    intro.
-    admit.
-  - asimpl.
-    assert (Hi : i < length fs). rewrite -Hfs; apply lookup_lt_is_Some; by econstructor.
-    destruct (fs !! i) eqn:Hf.
-    + rewrite (env_subst_lookup fs _ v).
-      apply ve_closed.
-      eapply (Forall_lookup_1). apply Hfsc. apply Hf. apply Hf.
-    + exfalso.
-      assert (length fs ≤ i). by apply lookup_ge_None_1.
-      lia.
-Admitted.
+  intro σ. rewrite /𝓕c. cut ((𝓕 pC).[upn 0 (env_subst fs)].[upn 0 σ] = (𝓕 pC).[upn 0 (env_subst fs)]). by asimpl.
+  by apply 𝓕c_closed_gen.
+Qed.
