theories/cast_calculus/consistency/standard.v
@@ -2,31 +2,85 @@ From Autosubst Require Export Autosubst.
 From fae_gtlc_mu Require Import prelude cast_calculus.types.
 Require Coq.Logic.JMeq.
 
-Inductive cons_stand : type -> type -> Type :=
-| GenSymUnit : cons_stand TUnit TUnit
-| GenSymUnknownL (τ : type) : cons_stand ⋆ τ
-| GenSymUnknownR (τ : type) : cons_stand τ ⋆
+From stdpp Require Import base list.
+From Autosubst Require Export Autosubst.
+Require Export Utf8_core.
+
+Inductive cons_stand_open : type -> type -> Type :=
+| GenSymUnit :
+    cons_stand_open TUnit TUnit
+| GenSymUnknownL τ :
+    cons_stand_open TUnknown τ
+| GenSymUnknownR τ :
+    cons_stand_open τ TUnknown
 | GenSymSum
     (τ1 τ1' τ2 τ2' : type)
-    (s1 : cons_stand τ1 τ1')
-    (s2 : cons_stand τ2 τ2')
-  : cons_stand (τ1 + τ2)%type (τ1' + τ2')%type
+    (s1 : cons_stand_open τ1 τ1')
+    (s2 : cons_stand_open τ2 τ2')
+  : cons_stand_open (τ1 + τ2)%type (τ1' + τ2')%type
 | GenSymProd
     (τ1 τ1' τ2 τ2' : type)
-    (s1 : cons_stand τ1 τ1')
-    (s2 : cons_stand τ2 τ2')
-  : cons_stand (τ1 × τ2) (τ1' × τ2')
-| GenSymArrow
-    (τ1 τ1' τ2 τ2' : type)
-    (s1 : cons_stand τ1 τ1')
-    (s2 : cons_stand τ2 τ2')
-  : cons_stand (TArrow τ1 τ2) (TArrow τ1' τ2')
-| GenSymVar (i : nat) :
-    cons_stand (TVar i) (TVar i)
-| GenSymRec (τ τ' : type) (P : cons_stand τ τ') :
-    cons_stand (TRec τ) (TRec τ').
+    (s1 : cons_stand_open τ1 τ1')
+    (s2 : cons_stand_open τ2 τ2')
+  : cons_stand_open (τ1 × τ2) (τ1' × τ2')
+| GenSymArrow τ1 τ1' τ2 τ2'
+    (s1 : cons_stand_open τ1 τ1')
+    (s2 : cons_stand_open τ2 τ2')
+  : cons_stand_open (TArrow τ1 τ2) (TArrow τ1' τ2')
+| GenSymVar i :
+    cons_stand_open (TVar i) (TVar i)
+| GenSymRec τ τ' (P : cons_stand_open τ τ') :
+    cons_stand_open (TRec τ) (TRec τ').
 
+Lemma cons_stand_open_sym {τ τ'} : cons_stand_open τ τ' → cons_stand_open τ' τ.
+Proof. induction 1; try by constructor. Qed.
 
-Lemma cons_stand_dec τ1 τ2 : TDecision (cons_stand τ1 τ2).
+Lemma cons_stand_open_unfold_help τ τ' α (pα : TClosed α) α' (pα' : TClosed α') k :
+  cons_stand_open (TRec τ) (TRec τ') → cons_stand_open α α' → cons_stand_open τ.[upn k (α .: ids)] τ'.[upn k (α' .: ids)].
 Proof.
-Admitted.
+  intro pC. inversion_clear pC.
+  generalize dependent τ'.
+  generalize dependent k.
+  induction τ.
+  - intros k τ' pC. inversion_clear pC.
+    + asimpl; constructor.
+    + asimpl; constructor.
+  - intros k τ' pC. inversion_clear pC.
+    + asimpl; constructor.
+    + asimpl; constructor. by apply IHτ1. by apply IHτ2.
+  - intros k τ' pC. inversion_clear pC.
+    + asimpl; constructor.
+    + asimpl; constructor. by apply IHτ1. by apply IHτ2.
+  - intros k τ' pC. inversion_clear pC.
+    + asimpl; constructor.
+    + asimpl; constructor. by apply IHτ1. by apply IHτ2.
+  - intros k τ' pC. inversion_clear pC.
+    + asimpl; constructor.
+    + intro. apply GenSymRec.
+      assert (triv : up (upn k (α .: ids)) = upn (S k) (α .: ids)); first by asimpl. rewrite triv.
+      by apply IHτ.
+  - intros k τ' pC. inversion_clear pC.
+    + asimpl; constructor.
+    + intro.
+      destruct (subst_fv_upn_cases x k (α .: ids)) as [[-> plt] | [j [eq ->]] ];
+      destruct (subst_fv_upn_cases x k (α' .: ids)) as [[-> plt'] | [j' [eq' ->]]]; try by (exfalso; lia).
+      * apply GenSymVar.
+      * assert (triv : j' = j). lia. rewrite triv. clear triv.
+        destruct j; asimpl. by rewrite pα pα'. apply GenSymVar.
+  - intros k τ' pC.
+    asimpl; constructor.
+Qed.
+
+Lemma cons_stand_open_unfold τ (pτ : TClosed (TRec τ)) τ' (pτ' : TClosed (TRec τ')) : cons_stand_open (TRec τ) (TRec τ') → cons_stand_open τ.[TRec τ/] τ'.[TRec τ'/].
+Proof.
+  intro pC.
+  assert (triv : τ.[TRec τ/] = τ.[upn 0 (TRec τ .: ids)]). by asimpl. rewrite triv. clear triv.
+  assert (triv : τ'.[TRec τ'/] = τ'.[upn 0 (TRec τ' .: ids)]). by asimpl. rewrite triv. clear triv.
+  by apply cons_stand_open_unfold_help; auto.
+Qed.
+
+Definition cons_stand τ (pτ : TClosed τ) τ' (pτ' : TClosed τ') : Type := cons_stand_open τ τ'.
+
+(* Lemma cons_stand_dec τ1 τ2 : TDecision (cons_stand τ1 τ2). *)
+(* Proof. *)
+(* Admitted. *)
