theories/stlc_mu/lib/fix.v
@@ -1,201 +1,43 @@
 From fae_gtlc_mu Require Export stlc_mu.lang.
 From fae_gtlc_mu Require Export stlc_mu.typing.
 
-Definition Fix : expr :=
-  Lam (
-      (Lam (Var 1 (Lam ((Unfold (Var 1)) (Var 1) (Var 0)))))
-        (Fold (Lam (Var 1 (Lam ((Unfold (Var 1)) (Var 1) (Var 0))))))
-  ).
-
-Definition Fix_typed Γ τa τr (pa : Is_Closed τa) (pr : Is_Closed τr) :
-  (Γ ⊢ₛ Fix : (TArrow (TArrow (TArrow τa τr) (TArrow τa τr)) (TArrow τa τr))).
-Proof.
-  apply Lam_typed.
-  apply App_typed with (τ1 := (TRec (TArrow (TVar 0) (TArrow τa τr)))).
-  - apply Lam_typed.
-    apply App_typed with (τ1 := TArrow τa τr); first by apply Var_typed.
-    apply Lam_typed.
-    apply App_typed with (τ1 := τa).
-    + apply App_typed with (τ1 := TRec (TArrow (TVar 0) (TArrow τa τr))).
-      apply Unfold_typed_help_2 with (τ := TArrow (TVar 0) (TArrow τa τr)).
-      asimpl. by rewrite pa pr. by apply Var_typed. by apply Var_typed.
-    + by apply Var_typed.
-  - apply Fold_typed. asimpl. rewrite pa pr.
-    apply Lam_typed.
-    apply App_typed with (τ1 := (TArrow τa τr)); first by apply Var_typed.
-    apply Lam_typed.
-    apply App_typed with (τ1 := τa).
-    apply App_typed with (τ1 := TRec (TArrow (TVar 0) (TArrow τa τr))).
-    apply Unfold_typed_help_2 with (τ := TArrow (TVar 0) (TArrow τa τr)).
-    asimpl. by rewrite pa pr. by apply Var_typed. by apply Var_typed.
-    by apply Var_typed.
-Qed.
-
-(* avoid to much substitutions since autosubst is as slow as a snail *)
-
-Definition Fix' (f : expr) : expr :=
-  (Lam ((rename (+1) f) (Lam ((Unfold (Var 1)) (Var 1) (Var 0)))))
-    (Fold (Lam (rename (+1) f (Lam ((Unfold (Var 1)) (Var 1) (Var 0)))))).
-
-Lemma Fix'_typed Γ τa τr f (pa : Is_Closed τa) (pr : Is_Closed τr) :
-  (Γ ⊢ₛ f : (TArrow (TArrow τa τr) (TArrow τa τr))) -> (Γ ⊢ₛ Fix' f : (TArrow τa τr)).
-Proof.
-  intros H.
-  apply App_typed with (τ1 := (TRec (TArrow (TVar 0) (TArrow τa τr)))).
-  - apply Lam_typed.
-    apply App_typed with (τ1 := TArrow τa τr). asimpl. rewrite -rename_ren. apply up_type_one. apply H.
-    apply Lam_typed.
-    apply App_typed with (τ1 := τa).
-    + apply App_typed with (τ1 := TRec (TArrow (TVar 0) (TArrow τa τr))).
-      asimpl. apply Unfold_typed_help_2 with (τ := TArrow (TVar 0) (TArrow τa τr)).
-      asimpl. by rewrite pa pr. by apply Var_typed. by apply Var_typed.
-    + by apply Var_typed.
-  - apply Fold_typed. asimpl. rewrite pa pr.
-    apply Lam_typed.
-    apply App_typed with (τ1 := (TArrow τa τr)). rewrite -rename_ren. apply up_type_one. apply H.
-    apply Lam_typed.
-    apply App_typed with (τ1 := τa).
-    apply App_typed with (τ1 := TRec (TArrow (TVar 0) (TArrow τa τr))).
-    + apply Unfold_typed_help_2 with (τ := (TArrow (TVar 0) (TArrow τa τr))).
-      asimpl. by rewrite pa pr. by apply Var_typed.
-    + by apply Var_typed.
-    + by apply Var_typed.
-Qed.
-
-Lemma Fix'_subs_rewrite f σ : (Fix' f).[σ] = Fix' (f.[σ]).
-Proof.
-  rewrite /Fix'.
-  by asimpl.
-Qed.
-
-Definition Fix'' (f : expr) : expr :=
+Definition Fix (f : expr) : expr :=
   (Unfold (Fold (Lam ((rename (+1) f) (Lam ((Unfold (Var 1)) (Var 1) (Var 0)))))))
     (Fold (Lam (rename (+1) f (Lam ((Unfold (Var 1)) (Var 1) (Var 0)))))).
 
-Lemma Fix''_typed Γ τa τr f (pa : Is_Closed τa) (pr : Is_Closed τr) :
-  (Γ ⊢ₛ f : (TArrow (TArrow τa τr) (TArrow τa τr))) -> (Γ ⊢ₛ Fix'' f : (TArrow τa τr)).
+(* Program Definition tau1 τa: ctype := [(TRec (TArrow (TVar 0) (TArrow τa τr))) % _]. *)
+
+Lemma Fix_typed Γ pΓ τa pτa τr pτr f :
+  (Γ & pΓ ⊢ₛ f : (TArrow (TArrow τa τr) (TArrow τa τr)) & (TArrow_closed (TArrow_closed pτa pτr) (TArrow_closed pτa pτr)))
+  -> (Γ & pΓ ⊢ₛ Fix f : (TArrow τa τr) & (TArrow_closed pτa pτr)).
 Proof.
   intros H.
-  apply App_typed with (τ1 := (TRec (TArrow (TVar 0) (TArrow τa τr)))).
-  - apply Unfold_typed_help_2 with (τ := TArrow (TVar 0) (TArrow τa τr)). by asimpl; by rewrite pa pr.
-    apply Fold_typed.
-    apply Lam_typed.
-    apply App_typed with (τ1 := TArrow τa τr). asimpl. rewrite -rename_ren. apply up_type_one.
-    rewrite pa pr.
-    apply H.
-    apply Lam_typed.
-    apply App_typed with (τ1 := τa).
-    + apply App_typed with (τ1 := TRec (TArrow (TVar 0) (TArrow τa τr))).
-      asimpl. apply Unfold_typed_help_2 with (τ := TArrow (TVar 0) (TArrow τa τr)).
-      asimpl. by rewrite pa pr. by apply Var_typed. by apply Var_typed.
+  eapply App_typed with (τ1 := (TRec (TArrow (TVar 0) (TArrow τa τr)))).
+  - apply Unfold_Fold_typed.
+    eapply Lam_typed.
+    eapply App_typed with (τ1 := TArrow τa τr). asimpl. by eapply up_type_one.
+    eapply Lam_typed.
+    eapply App_typed with (τ1 := τa).
+    + eapply App_typed with (τ1 := TRec (TArrow (TVar 0) (TArrow τa τr))).
+      asimpl. eapply Unfold_typed_help with (τb := TArrow (TVar 0) (TArrow τa τr)).
+      asimpl. by rewrite pτa pτr. by apply Var_typed. by apply Var_typed.
     + by apply Var_typed.
-  - apply Fold_typed. asimpl. rewrite pa pr.
-    apply Lam_typed.
-    apply App_typed with (τ1 := (TArrow τa τr)). rewrite -rename_ren. apply up_type_one. apply H.
-    apply Lam_typed.
-    apply App_typed with (τ1 := τa).
-    apply App_typed with (τ1 := TRec (TArrow (TVar 0) (TArrow τa τr))).
-    + apply Unfold_typed_help_2 with (τ := (TArrow (TVar 0) (TArrow τa τr))).
-      asimpl. by rewrite pa pr. by apply Var_typed.
+  - eapply Fold_typed. asimpl.
+    eapply Lam_typed.
+    eapply App_typed with (τ1 := (TArrow τa τr)). eapply up_type_one. eapply (rewrite_typed H). by rewrite pτa pτr.
+    eapply Lam_typed.
+    eapply App_typed with (τ1 := τa).
+    eapply App_typed with (τ1 := TRec (TArrow (TVar 0) (TArrow τa τr))).
+    + eapply Unfold_typed_help with (τb := (TArrow (TVar 0) (TArrow τa τr))).
+      asimpl. by rewrite pτa pτr. by apply Var_typed.
     + by apply Var_typed.
     + by apply Var_typed.
+      Unshelve. 1-24:intro σ; asimpl; by repeat rewrite pτa pτr.
 Qed.
 
-Lemma Fix''_subs_rewrite f σ : (Fix'' f).[σ] = Fix'' (f.[σ]).
+
+Lemma Fix_subs_rewrite f σ : (Fix f).[σ] = Fix (f.[σ]).
 Proof.
-  rewrite /Fix''.
+  rewrite /Fix.
   by asimpl.
 Qed.
-
-(* Definition Fix'' (f : expr) : expr := *)
-(*   (Lam (f (Lam ((Unfold (Var 1)) (Var 1) (Var 0))))) *)
-(*     (Fold (Lam (f (Lam ((Unfold (Var 1)) (Var 1) (Var 0)))))). *)
-
-(* (* Lemma Fix''_typed Γ τa τr f (pa : Is_Closed τa) (pr : Is_Closed τr) : *) *)
-(* (*   (Γ ⊢ₛ f : (TArrow (TArrow τa τr) (TArrow τa τr))) -> (Γ ⊢ₛ Fix'' f : (TArrow τa τr)). *) *)
-(* (* Proof. *) *)
-(* (*   intros H. *) *)
-(* (*   apply App_typed with (τ1 := (TRec (TArrow (TVar 0) (TArrow τa τr)))). *) *)
-(* (*   - apply Lam_typed. *) *)
-(* (*     apply App_typed with (τ1 := TArrow τa τr). asimpl. rewrite -rename_ren. apply up_type_one. apply H. *) *)
-(* (*     apply Lam_typed. *) *)
-(* (*     apply App_typed with (τ1 := τa). *) *)
-(* (*     + apply App_typed with (τ1 := TRec (TArrow (TVar 0) (TArrow τa τr))). *) *)
-(* (*       asimpl. apply Unfold_typed_help_2 with (τ := TArrow (TVar 0) (TArrow τa τr)). *) *)
-(* (*       asimpl. by rewrite pa pr. by apply Var_typed. by apply Var_typed. *) *)
-(* (*     + by apply Var_typed. *) *)
-(* (*   - apply Fold_typed. asimpl. rewrite pa pr. *) *)
-(* (*     apply Lam_typed. *) *)
-(* (*     apply App_typed with (τ1 := (TArrow τa τr)). rewrite -rename_ren. apply up_type_one. apply H. *) *)
-(* (*     apply Lam_typed. *) *)
-(* (*     apply App_typed with (τ1 := τa). *) *)
-(* (*     apply App_typed with (τ1 := TRec (TArrow (TVar 0) (TArrow τa τr))). *) *)
-(* (*     + apply Unfold_typed_help_2 with (τ := (TArrow (TVar 0) (TArrow τa τr))). *) *)
-(* (*       asimpl. by rewrite pa pr. by apply Var_typed. *) *)
-(* (*     + by apply Var_typed. *) *)
-(* (*     + by apply Var_typed. *) *)
-(* (* Qed. *) *)
-
-(* Lemma test0 σ : (Var 0).[ids 0 .: σ] = Var 0. *)
-(* Proof. *)
-(*   by simpl. *)
-(* Qed. *)
-
-(* Lemma test1 σ : (Var 0).[ids 0 .: σ] = (Var 0). *)
-(* Proof. *)
-(*   asimpl. done. *)
-(* Qed. *)
-
-(* Lemma test2 e σ : (rename (+1) e).[ids 0 .: σ] = e.[σ]. *)
-(* Proof. *)
-(*   asimpl. done. *)
-(* Qed. *)
-
-Definition Fix_stepped : expr :=
-  (Lam (Var 1 (Lam ((Unfold (Var 1)) (Var 1) (Var 0)))))
-    (Fold (Lam (Var 1 (Lam ((Unfold (Var 1)) (Var 1) (Var 0)))))).
-
-
-Definition Fix_stepped_subs_typed Γ τa τr f (pa : Is_Closed τa) (pr : Is_Closed τr) :
-  (Γ ⊢ₛ f : (TArrow (TArrow τa τr) (TArrow τa τr))) -> (Γ ⊢ₛ Fix_stepped.[f/] : (TArrow τa τr)).
-Proof.
-  intros H.
-  apply App_typed with (τ1 := (TRec (TArrow (TVar 0) (TArrow τa τr)))).
-  - apply Lam_typed.
-    apply App_typed with (τ1 := TArrow τa τr). asimpl. rewrite -rename_ren. apply up_type_one. apply H.
-    apply Lam_typed.
-    apply App_typed with (τ1 := τa).
-    + apply App_typed with (τ1 := TRec (TArrow (TVar 0) (TArrow τa τr))).
-      asimpl. apply Unfold_typed_help_2 with (τ := TArrow (TVar 0) (TArrow τa τr)).
-      asimpl. by rewrite pa pr. by apply Var_typed. by apply Var_typed.
-    + by apply Var_typed.
-  - apply Fold_typed. asimpl. rewrite pa pr.
-    apply Lam_typed.
-    apply App_typed with (τ1 := (TArrow τa τr)). rewrite -rename_ren. apply up_type_one. apply H.
-    apply Lam_typed.
-    apply App_typed with (τ1 := τa).
-    apply App_typed with (τ1 := TRec (TArrow (TVar 0) (TArrow τa τr))).
-    + apply Unfold_typed_help_2 with (τ := (TArrow (TVar 0) (TArrow τa τr))).
-      asimpl. by rewrite pa pr. by apply Var_typed.
-    + by apply Var_typed.
-    + by apply Var_typed.
-Qed.
-
-(* Definition Fix_stepped_typed Γ τ : (Is_Closed τ) -> (((TArrow τ τ) :: Γ) ⊢ₛ Fix_stepped : τ). *)
-(* Proof. *)
-(*   intro P. *)
-(*   apply App_typed with (τ1 := (TRec (TArrow (TVar 0) τ))). *)
-(*   - apply Lam_typed. *)
-(*     apply App_typed with (τ1 := τ); first by apply Var_typed. *)
-(*     apply App_typed with (τ1 := TRec (TArrow (TVar 0) τ)). *)
-(*     + apply Unfold_typed_help_2 with (τ := TArrow (TVar 0) τ). *)
-(*       asimpl. by rewrite P. by apply Var_typed. *)
-(*     + by apply Var_typed. *)
-(*   - apply Fold_typed. asimpl. rewrite P. *)
-(*     apply Lam_typed. *)
-(*     apply App_typed with (τ1 := τ); first by apply Var_typed. *)
-(*     apply App_typed with (τ1 := TRec (TArrow (TVar 0) τ)). *)
-(*     + apply Unfold_typed_help_2 with (τ := (TArrow (TVar 0) τ)). *)
-(*       asimpl. by rewrite P. by apply Var_typed. *)
-(*     + by apply Var_typed. *)
-(* Qed. *)
