theories/backtranslation/cast_help/embed.v
@@ -10,12 +10,13 @@ Definition embedV_TUnit (v : val) : val :=
 Definition embed_TUnit : val :=
   LamV (Fold (InjL (InjL (InjL (InjL (Var 0)))))).
 
-Lemma embed_TUnit_typed Γ :
-  Γ ⊢ₛ embed_TUnit : (TArrow TUnit Universe).
+Lemma embed_TUnit_typed Γ pΓ :
+  Γ & pΓ ⊢ₛ embed_TUnit : (TArrow TUnit Universe) & (TArrow_closed TUnit_TClosed Universe_closed).
 Proof.
-  apply Lam_typed, Fold_typed.
-  repeat apply InjL_typed.
-  by apply Var_typed.
+  eapply Lam_typed, Fold_typed.
+  repeat eapply InjL_typed.
+  by eapply Var_typed.
+  Unshelve. all:intro σ; by asimpl.
 Qed.
 
 Definition embedV_Ground_TSum (s : val) : val :=
@@ -24,13 +25,15 @@ Definition embedV_Ground_TSum (s : val) : val :=
 Definition embed_Ground_TSum : val :=
   LamV (Fold ((InjL (InjL (InjL (InjR (Var 0))))))).
 
-Definition embed_Ground_TSum_typed Γ :
-  Γ ⊢ₛ embed_Ground_TSum : (TArrow (Universe + Universe) Universe)%type.
+Definition embed_Ground_TSum_typed Γ pΓ :
+  Γ & pΓ ⊢ₛ embed_Ground_TSum : (TArrow (Universe + Universe) Universe)%type &
+                                (TArrow_closed (TSum_closed Universe_closed Universe_closed) Universe_closed).
 Proof.
-  apply Lam_typed.
-  apply Fold_typed.
-  repeat apply InjL_typed. apply InjR_typed.
+  eapply Lam_typed.
+  eapply Fold_typed.
+  repeat eapply InjL_typed. eapply InjR_typed.
   by apply Var_typed.
+  Unshelve. all:intro σ; by asimpl.
 Qed.
 
 Definition embedV_Ground_TProd (p : val) : val :=
@@ -39,12 +42,14 @@ Definition embedV_Ground_TProd (p : val) : val :=
 Definition embed_Ground_TProd : val :=
   LamV (Fold (InjL (InjL (InjR (Var 0))))).
 
-Definition embed_Ground_TProd_typed Γ :
-  Γ ⊢ₛ embed_Ground_TProd : (TArrow (Universe × Universe) Universe).
+Definition embed_Ground_TProd_typed Γ pΓ :
+  Γ & pΓ ⊢ₛ embed_Ground_TProd : (TArrow (Universe × Universe) Universe) &
+                                 ltac:(apply (TArrow_closed (TProd_closed Universe_closed Universe_closed) Universe_closed)).
 Proof.
-  apply Lam_typed, Fold_typed.
-  repeat apply InjL_typed. asimpl. repeat apply InjR_typed.
+  eapply Lam_typed, Fold_typed.
+  repeat eapply InjL_typed. asimpl. repeat eapply InjR_typed.
   by apply Var_typed.
+  Unshelve. all:intro σ; by asimpl.
 Qed.
 
 Definition embedV_Ground_TArrow (v : val) : val :=
@@ -53,12 +58,14 @@ Definition embedV_Ground_TArrow (v : val) : val :=
 Definition embed_Ground_TArrow : val :=
   LamV (Fold (InjL (InjR (Var 0)))).
 
-Definition embed_Ground_TArrow_typed Γ :
-  Γ ⊢ₛ embed_Ground_TArrow : (TArrow (TArrow Universe Universe) Universe).
+Definition embed_Ground_TArrow_typed Γ pΓ :
+  Γ & pΓ ⊢ₛ embed_Ground_TArrow : (TArrow (TArrow Universe Universe) Universe) &
+                                  (TArrow_closed (TArrow_closed Universe_closed Universe_closed) Universe_closed).
 Proof.
-  apply Lam_typed, Fold_typed.
-  repeat apply InjL_typed. asimpl. repeat apply InjR_typed.
+  eapply Lam_typed, Fold_typed.
+  repeat eapply InjL_typed. asimpl. repeat eapply InjR_typed.
   by apply Var_typed.
+  Unshelve. all:intro σ; by asimpl.
 Qed.
 
 (* Takes something of μ.Universe, unfolds it so it is in Universe, and then puts in the last branch of the universe *)
@@ -66,15 +73,20 @@ Qed.
 Definition embed_Ground_TRec : val :=
   LamV (Fold (InjR (Unfold (Var 0)))).
 
-Definition embed_Ground_TRec_typed Γ :
-  Γ ⊢ₛ embed_Ground_TRec : (TArrow (TRec Universe) Universe).
+Definition embed_Ground_TRec_typed Γ pΓ :
+  Γ & pΓ ⊢ₛ embed_Ground_TRec : (TArrow (TRec Universe) Universe) &
+                                (TArrow_closed (TRec_closed Universe_closed) Universe_closed).
 Proof.
-  apply Lam_typed. apply Fold_typed.
-  apply InjR_typed.
+  eapply Lam_typed. eapply Fold_typed.
+  eapply InjR_typed.
   asimpl.
-  apply Unfold_typed_help; first by trivial.
+  eapply Unfold_typed_help with (τb := Universe). by rewrite Universe_closed.
   by apply Var_typed.
+  Unshelve. all:intro σ; by asimpl.
 Qed.
+
+Definition embedV_TUnknown (u : val) : val := (** a bit different from the other ones... u : Universe instead of u : μX.Universe *)
+  (FoldV (InjRV u)).
 
 Definition embed (τ : cast_calculus.types.type) (G : Ground τ) : val :=
   match G with
@@ -85,10 +97,11 @@ Definition embed (τ : cast_calculus.types.type) (G : Ground τ) : val :=
   | Ground_TRec => embed_Ground_TRec
   end.
 
-Lemma embed_typed {τG : cast_calculus.types.type} {G : Ground τG} Γ :
-  Γ ⊢ₛ (embed τG G) : (TArrow <<τG>> Universe).
+Lemma embed_typed {τG : cast_calculus.types.type} {G : Ground τG} Γ pΓ :
+  Γ & pΓ ⊢ₛ (embed τG G) : (TArrow <<τG>> Universe) &
+                           (TArrow_closed (back_Ground_closed G) Universe_closed).
 Proof.
-  destruct G.
+  destruct G; eapply PI_typed.
     + apply embed_TUnit_typed.
     + apply embed_Ground_TProd_typed.
     + apply embed_Ground_TSum_typed.
@@ -100,3 +113,4 @@ Lemma embed_no_subs {τ : cast_calculus.types.type} {G : Ground τ} σ : (# (emb
 Proof.
   destruct G; by asimpl.
 Qed.
+
