theories/backtranslation/cast_help/extract.v
@@ -10,21 +10,21 @@ Definition Ω : expr :=
       (Fold (Lam ((Unfold (Var 0)) (Var 0))))
   ).
 
-Definition Ω_typed Γ τ : (Is_Closed τ) -> (Γ ⊢ₛ Ω : τ).
+Definition Ω_typed Γ pΓ τ pτ : Γ & pΓ ⊢ₛ Ω : τ & pτ.
 Proof.
-  intro P.
-  apply App_typed with (τ1 := (TRec (TArrow (TVar 0) τ))).
-  - apply Lam_typed.
-    apply App_typed with (τ1 := TRec (TArrow (TVar 0) τ)).
-    + apply Unfold_typed_help_2 with (τ := (TArrow (TVar 0) τ)).
-      asimpl. by rewrite P. by apply Var_typed.
+  eapply App_typed with (τ1 := (TRec (TArrow (TVar 0) τ))).
+  - eapply Lam_typed.
+    eapply App_typed with (τ1 := TRec (TArrow (TVar 0) τ)).
+    + eapply Unfold_typed_help with (τb := (TArrow (TVar 0) τ)).
+      asimpl. by rewrite pτ. by apply Var_typed.
     + by apply Var_typed.
-  - apply Fold_typed. asimpl. rewrite P.
-    apply Lam_typed.
-    apply App_typed with (τ1 := TRec (TArrow (TVar 0) τ)).
-    + apply Unfold_typed_help_2 with (τ := (TArrow (TVar 0) τ)).
-      asimpl. by rewrite P. by apply Var_typed.
+  - eapply Fold_typed. asimpl.
+    eapply Lam_typed.
+    eapply App_typed with (τ1 := TRec (TArrow (TVar 0) τ)).
+    + eapply Unfold_typed_help with (τb := (TArrow (TVar 0) τ)).
+      by asimpl. by apply Var_typed.
     + by apply Var_typed.
+    Unshelve. 1-13:intro σ; asimpl; by repeat rewrite pτ.
 Qed.
 
 Definition extract_TUnit : val :=
@@ -42,14 +42,15 @@ Definition extract_TUnit : val :=
             (Ω)
       ).
 
-Definition extract_TUnit_typed Γ : Γ ⊢ₛ extract_TUnit : (TArrow Universe TUnit).
+Definition extract_TUnit_typed Γ pΓ: Γ & pΓ ⊢ₛ extract_TUnit : (TArrow Universe TUnit) &
+                                                                (TArrow_closed Universe_closed TUnit_TClosed).
 Proof.
-  apply Lam_typed.
-  apply Case_typed with (τ1 := (TUnit + (TVar 0 + TVar 0) + (TVar 0 × TVar 0) + (TArrow (TVar 0) (TVar 0))).[Universe/]%type)
+  eapply Lam_typed.
+  eapply Case_typed with (τ1 := (TUnit + (TVar 0 + TVar 0) + (TVar 0 × TVar 0) + (TArrow (TVar 0) (TVar 0))).[Universe/]%type)
                          (τ2 := Universe).
-  - eapply Unfold_typed_help_2 with (τ := Universe_body). by asimpl.
+  - eapply Unfold_typed_help with (τb := Universe_body). by asimpl.
     by apply Var_typed.
-  - apply Case_typed with (τ1 := (TUnit + (TVar 0 + TVar 0) + (TVar 0 × TVar 0)).[Universe/]%type)
+  - eapply Case_typed with (τ1 := (TUnit + (TVar 0 + TVar 0) + (TVar 0 × TVar 0)).[Universe/]%type)
                           (τ2 := (TArrow (TVar 0) (TVar 0)).[Universe/]%type).
     + by apply Var_typed.
     + eapply Case_typed.
@@ -61,6 +62,7 @@ Proof.
       * by apply Ω_typed.
     + by apply Ω_typed.
   - by apply Ω_typed.
+  Unshelve. all:intro σ; by asimpl.
 Qed.
 
 Definition extract_Ground_TSum : val :=
@@ -78,12 +80,13 @@ Definition extract_Ground_TSum : val :=
             (Ω)
       ).
 
-Definition extract_Ground_TSum_typed Γ : Γ ⊢ₛ extract_Ground_TSum : (TArrow Universe (Universe + Universe))%type.
+Definition extract_Ground_TSum_typed Γ pΓ: Γ & pΓ ⊢ₛ extract_Ground_TSum : (TArrow Universe (Universe + Universe))%type &
+                                                                           (TArrow_closed Universe_closed (TSum_closed Universe_closed Universe_closed)).
 Proof.
-  apply Lam_typed.
-  apply Case_typed with (τ1 := (TUnit + (TVar 0 + TVar 0) + (TVar 0 × TVar 0) + (TArrow (TVar 0) (TVar 0))).[Universe/]%type)
+  eapply Lam_typed.
+  eapply Case_typed with (τ1 := (TUnit + (TVar 0 + TVar 0) + (TVar 0 × TVar 0) + (TArrow (TVar 0) (TVar 0))).[Universe/]%type)
                          (τ2 := Universe).
-  - eapply Unfold_typed_help_2 with (τ := Universe_body). by asimpl. by apply Var_typed.
+  - eapply Unfold_typed_help with (τb := Universe_body). by asimpl. by apply Var_typed.
   - eapply Case_typed. by apply Var_typed.
     + eapply Case_typed.
       * by apply Var_typed.
@@ -94,7 +97,9 @@ Proof.
       * by apply Ω_typed.
     + by apply Ω_typed.
   - by apply Ω_typed.
+  Unshelve. all:intro σ; by asimpl.
 Qed.
+
 
 Definition extract_Ground_TProd : val :=
   LamV (Case (Unfold (Var 0))
@@ -108,12 +113,13 @@ Definition extract_Ground_TProd : val :=
             (Ω)
       ).
 
-Definition extract_Ground_TProd_typed Γ : Γ ⊢ₛ extract_Ground_TProd : (TArrow Universe (Universe × Universe)).
+Definition extract_Ground_TProd_typed Γ pΓ: Γ & pΓ ⊢ₛ extract_Ground_TProd : (TArrow Universe (Universe × Universe)) &
+ (TArrow_closed Universe_closed (TProd_closed Universe_closed Universe_closed)).
 Proof.
-  apply Lam_typed.
-  apply Case_typed with (τ1 := (TUnit + (TVar 0 + TVar 0) + (TVar 0 × TVar 0) + (TArrow (TVar 0) (TVar 0))).[Universe/]%type)
+  eapply Lam_typed.
+  eapply Case_typed with (τ1 := (TUnit + (TVar 0 + TVar 0) + (TVar 0 × TVar 0) + (TArrow (TVar 0) (TVar 0))).[Universe/]%type)
                          (τ2 := Universe).
-  - eapply Unfold_typed_help_2 with (τ := Universe_body). by asimpl. by apply Var_typed.
+  - eapply Unfold_typed_help with (τb := Universe_body). by asimpl. by apply Var_typed.
   - eapply Case_typed. by apply Var_typed.
     + eapply Case_typed.
       * by apply Var_typed.
@@ -121,7 +127,9 @@ Proof.
       * by apply Var_typed.
     + by apply Ω_typed.
   - by apply Ω_typed.
+  Unshelve. all:intro σ; by asimpl.
 Qed.
+
 
 Definition extract_Ground_TArrow : val :=
   LamV (Case (Unfold (Var 0))
@@ -132,17 +140,20 @@ Definition extract_Ground_TArrow : val :=
             (Ω)
       ).
 
-Definition extract_Ground_TArrow_typed Γ : Γ ⊢ₛ extract_Ground_TArrow : (TArrow Universe (TArrow Universe Universe)).
+Definition extract_Ground_TArrow_typed Γ pΓ: Γ & pΓ ⊢ₛ extract_Ground_TArrow : (TArrow Universe (TArrow Universe Universe)) &
+TArrow_closed Universe_closed (TArrow_closed Universe_closed Universe_closed).
 Proof.
-  apply Lam_typed.
-  apply Case_typed with (τ1 := (TUnit + (TVar 0 + TVar 0) + (TVar 0 × TVar 0) + (TArrow (TVar 0) (TVar 0))).[Universe/]%type)
+  eapply Lam_typed.
+  eapply Case_typed with (τ1 := (TUnit + (TVar 0 + TVar 0) + (TVar 0 × TVar 0) + (TArrow (TVar 0) (TVar 0))).[Universe/]%type)
                          (τ2 := Universe).
-  - eapply Unfold_typed_help_2 with (τ := Universe_body). by asimpl. by apply Var_typed.
+  - eapply Unfold_typed_help with (τb := Universe_body). by asimpl. by apply Var_typed.
   - eapply Case_typed. by apply Var_typed.
     + by apply Ω_typed.
     + by apply Var_typed.
   - by apply Ω_typed.
+  Unshelve. all:intro σ; by asimpl.
 Qed.
+
 
 Definition extract_Ground_TRec : val :=
   LamV (Case (Unfold (Var 0))
@@ -150,16 +161,18 @@ Definition extract_Ground_TRec : val :=
             (Fold (Var 0))
       ).
 
-Definition extract_Ground_TRec_typed Γ : Γ ⊢ₛ extract_Ground_TRec : (TArrow Universe (TRec Universe)).
+Definition extract_Ground_TRec_typed Γ pΓ: Γ & pΓ ⊢ₛ extract_Ground_TRec : (TArrow Universe (TRec Universe)) &
+TArrow_closed Universe_closed (TRec_closed Universe_closed).
 Proof.
-  apply Lam_typed.
-  apply Case_typed with (τ1 := (TUnit + (TVar 0 + TVar 0) + (TVar 0 × TVar 0) + (TArrow (TVar 0) (TVar 0))).[Universe/]%type)
+  eapply Lam_typed.
+  eapply Case_typed with (τ1 := (TUnit + (TVar 0 + TVar 0) + (TVar 0 × TVar 0) + (TArrow (TVar 0) (TVar 0))).[Universe/]%type)
 
 
                         (τ2 := Universe).
-  - eapply Unfold_typed_help_2 with (τ := Universe_body). by asimpl. by apply Var_typed.
+  - eapply Unfold_typed_help with (τb := Universe_body). by asimpl. by apply Var_typed.
   - by apply Ω_typed.
-  - apply Fold_typed. by apply Var_typed.
+  - eapply Fold_typed. by apply Var_typed.
+    Unshelve. 1-7:intro σ; by asimpl.
 Qed.
 
 Definition extract (τ : cast_calculus.types.type) (G : Ground τ) : val :=
@@ -171,10 +184,11 @@ Definition extract (τ : cast_calculus.types.type) (G : Ground τ) : val :=
   | Ground_TRec => extract_Ground_TRec
   end.
 
-Lemma extract_typed {τG : cast_calculus.types.type} {G : Ground τG} Γ :
-  Γ ⊢ₛ (extract τG G) : (TArrow Universe <<τG>>).
+Lemma extract_typed {τG : cast_calculus.types.type} {G : Ground τG} Γ pΓ:
+  Γ & pΓ ⊢ₛ (extract τG G) : (TArrow Universe <<τG>>) &
+TArrow_closed Universe_closed (back_Ground_closed G).
 Proof.
-  destruct G.
+  destruct G; eapply PI_typed.
     + apply extract_TUnit_typed.
     + apply extract_Ground_TProd_typed.
     + apply extract_Ground_TSum_typed.
