theories/backtranslation/types.v
@@ -12,7 +12,67 @@ Fixpoint backtranslate_type (τ : cast_calculus.types.type) : type :=
   | cast_calculus.types.TUnknown => Universe
   end where "<< e >>" := (backtranslate_type e).
 
-Lemma unfolding_backtranslation_commutes (τ : cast_calculus.types.type) :
-  << (cast_calculus.types.unfoldish τ) >> = stlc_mu.typing.unfoldish << τ >>.
+(* From stdpp Require Import base list. *)
+(* From Autosubst Require Export Autosubst. *)
+(* From iris Require Export base. *)
+(* Require Export Utf8_core. *)
+
+Lemma back_Ground_closed {τG} (G : Ground τG) : TClosed <<τG>>.
+Proof. destruct G; intro σ; simpl; by repeat rewrite Universe_closed. Qed.
+
+Lemma btype_ren_gen τ :
+  forall k l, << τ.[upn l (ren (+k))] >> = <<τ>>.[upn l (ren (+k))].
 Proof.
-Admitted.
+  induction τ; intros k l; try by asimpl.
+  - asimpl. by rewrite IHτ1 IHτ2.
+  - asimpl. by rewrite IHτ1 IHτ2.
+  - asimpl. by rewrite IHτ1 IHτ2.
+  - simpl. specialize (IHτ k (S l)). by rewrite IHτ.
+  - asimpl. do 2 rewrite (iter_up l x (ren (+k))).
+    destruct (lt_dec x l); by asimpl.
+Qed.
+
+Lemma back_unfold_comm_gen (τb : cast_calculus.types.type) : forall (τ : cast_calculus.types.type) k,
+  << τb.[upn k (τ .: ids)] >> = <<τb>>.[upn k (<<τ>> .: ids)].
+Proof.
+  induction τb; intros τ' k; try by asimpl.
+  - asimpl. by rewrite IHτb1 IHτb2.
+  - asimpl. by rewrite IHτb1 IHτb2.
+  - asimpl. by rewrite IHτb1 IHτb2.
+  - simpl. specialize (IHτb τ' (S k)). by rewrite IHτb.
+  - asimpl.
+    rewrite (iter_up k x (τ' .: ids)) (iter_up k x (<<τ'>> .: ids)).
+    destruct (lt_dec x k).
+      + by asimpl.
+      + destruct (decide (x - k = 0)); asimpl. rewrite e. asimpl.
+        cut (<< τ'.[upn 0 (ren (+k))] >> = (<< τ' >>).[upn 0 (ren (+k))]).
+        by asimpl. by rewrite btype_ren_gen.
+        destruct (x - k). exfalso; lia. by asimpl.
+Qed.
+
+Lemma back_unfold_comm (τb : cast_calculus.types.type) :
+  << τb.[cast_calculus.types.TRec τb/]>> = <<τb>>.[TRec <<τb>>/].
+Proof.
+  cut (<< (τb.[upn 0 ((cast_calculus.types.TRec τb) .: ids)])>> = <<τb>>.[upn 0 (<<(cast_calculus.types.TRec τb)>> .: ids)]).
+  by asimpl. apply back_unfold_comm_gen.
+Qed.
+
+Lemma back_closed_gen τ : forall n (pnτ : cast_calculus.types.TnClosed n τ), TnClosed n <<τ>>.
+Proof.
+  induction τ; intros n pnτ; simpl; try by (intro σ; by asimpl).
+  - specialize (IHτ1 n (cast_calculus.types.TProd_nclosed1 pnτ)).
+    specialize (IHτ2 n (cast_calculus.types.TProd_nclosed2 pnτ)).
+    intro σ; asimpl; by rewrite IHτ1 IHτ2.
+  - specialize (IHτ1 n (cast_calculus.types.TSum_nclosed1 pnτ)).
+    specialize (IHτ2 n (cast_calculus.types.TSum_nclosed2 pnτ)).
+    intro σ; asimpl; by rewrite IHτ1 IHτ2.
+  - specialize (IHτ1 n (cast_calculus.types.TArrow_nclosed1 pnτ)).
+    specialize (IHτ2 n (cast_calculus.types.TArrow_nclosed2 pnτ)).
+    intro σ; asimpl; by rewrite IHτ1 IHτ2.
+  - specialize (IHτ (S n) (cast_calculus.types.TRec_nclosed1 pnτ)).
+    intro σ; asimpl; by rewrite IHτ.
+  - apply TnClosed_var. by apply cast_calculus.types.TnClosed_var.
+Qed.
+
+Lemma back_closed {τ} (pτ : cast_calculus.types.TClosed τ) : TClosed <<τ>>.
+Proof. apply (back_closed_gen τ 0 pτ). Qed.
