theories/prelude.v
@@ -19,6 +19,27 @@ Section Autosubst_Lemmas.
     revert x; induction m as [|m IH]=> -[|x];
       repeat (destruct (lt_dec _ _) || asimpl || rewrite IH); auto with lia.
   Qed.
+
+
+  Lemma iter_up_cases k n σ : (upn n σ k = ids k ∧ k < n) +
+                                   { j : nat | (k = (n + j)%nat) ∧ upn n σ k = (σ j).[ren (+n)]  }.
+  Proof.
+    destruct (decide (k < n)).
+    - left. split. rewrite iter_up. destruct (lt_dec k n). auto. exfalso;lia. auto.
+    - apply inr. exists (k - n). split. lia. rewrite iter_up. destruct (lt_dec k n).
+      contradiction. by asimpl.
+  Qed.
+
+  Lemma upn_lt i n σ : i < n → upn n σ i = ids i.
+  Proof.
+    generalize dependent i.
+    induction n.
+    - intros. exfalso. lia.
+    - intros. destruct i.
+      + by asimpl.
+      + asimpl. rewrite IHn. by asimpl. lia.
+  Qed.
+
 End Autosubst_Lemmas.
 
 Inductive ForallT {A : Type} (P : A → Type) : list A → Type :=
